Typing rules IWrap/Unwrap: generate fresh type variables [squashed]

src/PlutusIR/Semantics/Static/Typing.v
@@ -46,7 +46,17 @@ Definition fromDecl (tvd : tvdecl) : string * kind :=
   | TyVarDecl v K => (v, K)
   end.
 
-Definition unwrapIFix (F : ty) (K : kind) (T : ty) : ty := (Ty_App (Ty_App F (Ty_Lam "X" K (Ty_IFix F (Ty_Var "X")))) T).
+Definition freshUnwrapIFix (F : ty) : string :=
+  "a" ++ String.concat EmptyString (FreeVars.Ty.ftv F).
+
+Definition unwrapIFix (F : ty) (K : kind) (T : ty) : ty :=
+  let b := freshUnwrapIFix F in
+  (Ty_App (Ty_App F (Ty_Lam b K (Ty_IFix F (Ty_Var b)))) T).
+
+(* Main property of fresh variables: they are fresh*)
+Lemma freshUnwrapIFix__fresh F :
+  ~ In (freshUnwrapIFix F) (FreeVars.Ty.ftv F).
+Admitted.
 
 (** Typing of terms *)
 Reserved Notation "Delta ',,' Gamma '|-+' t ':' T" (at level 101, t at level 0, T at level 0, no associativity).
